examples/iso_dh/proofs/base.v
@@ -4,14 +4,14 @@ From mathcomp Require ssrbool.
 From iris.algebra Require Import agree auth csum gset gmap excl frac.
 From iris.algebra Require Import reservation_map.
 From iris.heap_lang Require Import notation proofmode.
-From cryptis Require Import lib.
-From cryptis.lib Require Import gmeta nown saved_prop.
-From cryptis Require Import cryptis primitives tactics role.
-From cryptis.examples.iso_dh Require Import impl.
+From cryptis Require Import lib term cryptis primitives tactics.
+From cryptis Require Import role.
 
 Set Implicit Arguments.
 Unset Strict Implicit.
 Unset Printing Implicit Defensive.
+
+Definition iso_dhN := nroot.@"iso_dh".
 
 Record sess_info := SessInfo {
   si_init : sign_key;
@@ -29,82 +29,29 @@ Global Instance sess_info_inhabited : Inhabited sess_info :=
   populate (SessInfo inhabitant inhabitant
               inhabitant inhabitant inhabitant).
 
-Class iso_dhGpreS Σ := IsoDhGPreS {
-  iso_dhGpreS_meta : metaGS Σ;
-  iso_dhGpreS_pred : savedPredG Σ (sign_key * sign_key * sess_info * role);
-}.
-
-Local Existing Instance iso_dhGpreS_meta.
-Local Existing Instance iso_dhGpreS_pred.
-
-Class iso_dhGS Σ := IsoDhGS {
-  iso_dh_inG : iso_dhGpreS Σ;
-  iso_dh_name : gname;
-}.
-
-Local Existing Instance iso_dh_inG.
-
-Definition iso_dhΣ := #[
-  metaΣ;
-  savedPredΣ (sign_key * sign_key * sess_info * role)
-].
-
-Global Instance subG_iso_dhGpreS Σ : subG iso_dhΣ Σ → iso_dhGpreS Σ.
-Proof. solve_inG. Qed.
-
 Section Verif.
 
-Context `{!heapGS Σ, !cryptisGS Σ, !iso_dhGS Σ}.
+Context `{!heapGS Σ, !cryptisGS Σ}.
 Notation iProp := (iProp Σ).
 
 Implicit Types (rl : role) (t nI nR sI sR kS : term).
-Implicit Types (skI skR : sign_key) (failed : bool).
+Implicit Types (skI skR : sign_key).
+Implicit Types (γ γa γb : gname) (ok failed : bool).
+Implicit Types (ts : nat) (T : gset term).
 Implicit Types (si : sess_info).
-Implicit Types (N : namespace) (E : coPset).
-Implicit Types (φ : sign_key → sign_key → sess_info → role → iProp).
 
-Definition iso_dh_token E : iProp :=
-  gmeta_token iso_dh_name E.
+(*
 
-Definition iso_dh_pred N φ : iProp :=
-  nown iso_dh_name N
-    (saved_pred DfracDiscarded (λ '(skI, skR, si, rl), φ skI skR si rl)).
+A --> B: g^a; pkA
+B --> A: {g^a; g^b; pkA}@skB
+A --> B: {g^a; g^b; pkB}@skA
 
-Lemma iso_dh_pred_set N φ E :
-  ↑N ⊆ E →
-  iso_dh_token E ==∗ iso_dh_pred N φ ∗ iso_dh_token (E ∖ ↑N).
-Proof. by iIntros "%"; iApply nown_alloc. Qed.
+Result: derive_key [pkA; pkB; g^a; g^b; g^ab]
 
-Lemma iso_dh_token_difference E1 E2 :
-  E1 ⊆ E2 →
-  iso_dh_token E2 ⊣⊢ iso_dh_token E1 ∗ iso_dh_token (E2 ∖ E1).
-Proof. exact: gmeta_token_difference. Qed.
+*)
 
-Lemma iso_dh_token_drop E1 E2 :
-  E1 ⊆ E2 →
-  iso_dh_token E2 -∗ iso_dh_token E1.
-Proof. exact: gmeta_token_drop. Qed.
-
-Definition iso_dh_ready N skI skR si : iProp := ∀ φ,
-  iso_dh_pred N φ →
-  term_token (si_init_share si) (↑iso_dhN.@"ready") ={⊤}=∗
-    ▷ φ skI skR si Init.
-
-Lemma iso_dh_ready_alloc N skI skR si φ :
-  iso_dh_pred N φ -∗
-  φ skI skR si Init ={⊤}=∗
-  □ iso_dh_ready N skI skR si.
-Proof.
-iIntros "#N_φ φ_ts".
-iMod (escrowI nroot with "φ_ts []") as "#?".
-{ by iApply (term_token_switch (si_init_share si) (iso_dhN.@"ready")). }
-iIntros "!> !>  %φ' #N_φ' ready".
-iPoseProof (nown_valid_2 with "N_φ N_φ'") as "#valid".
-iPoseProof (saved_pred_op_validI with "valid") as "[_ #φ_eq]".
-iSpecialize ("φ_eq" $! (skI, skR, si, Init)).
-iMod (escrowE with "[//] ready") as "res" => //.
-iIntros "!> !>". by iRewrite -"φ_eq".
-Qed.
+Definition mk_keyshare : val := λ: "k",
+  texp (tint #0) "k".
 
 Lemma wp_mk_keyshare (t : term) :
   {{{ True }}}
@@ -117,7 +64,7 @@ wp_bind (texp _ _). iApply wp_texp.
 by iApply "Hpost".
 Qed.
 
-Definition iso_dh_key_share t : iProp :=
+Definition iso_dh_pred t : iProp :=
   ⌜length (exps t) = 1⌝.
 
 Definition si_key si : senc_key :=
@@ -139,12 +86,10 @@ rewrite /si_key /=. case => /Spec.of_list_inj.
 by case=> /Spec.sign_pkey_inj <- /Spec.sign_pkey_inj <- <- <- <-.
 Qed.
 
-Definition compromised si : iProp :=
+Definition compromised_session rl si : iProp :=
   (public (si_init si) ∨ public (si_resp si)) ∗
-  public (si_key si).
-
-Lemma compromised_public si : compromised si ⊢ public (si_key si).
-Proof. by iIntros "(_&?)". Qed.
+  public (si_key si) ∗
+  term_meta (si_share_of rl si) (iso_dhN.@"failed") true.
 
 Definition release_token share : iProp :=
   term_token share (↑iso_dhN.@"released").
@@ -163,17 +108,14 @@ Definition released share : iProp :=
 Lemma release share : release_token share ==∗ released share.
 Proof. by apply term_meta_set. Qed.
 
+Definition unreleased share : iProp :=
+  term_meta share (iso_dhN.@"released") false.
+
+Lemma unrelease share : release_token share ==∗ unreleased share.
+Proof. by apply term_meta_set. Qed.
+
 Definition released_session si : iProp :=
   released (si_init_share si) ∧ released (si_resp_share si).
-
-Lemma unrelease rl si : release_token (si_share_of rl si) ==∗ □ ¬ released_session si.
-Proof.
-iIntros "tok".
-iMod (term_meta_set (iso_dhN.@"released") false with "tok") as "#un" => //.
-iIntros "!> !> [#init #resp]".
-iAssert (released (si_share_of rl si)) as "r"; first by case: rl.
-by iPoseProof (term_meta_agree with "r un") as "%".
-Qed.
 
 Lemma release_token_released_session si rl :
   release_token (si_share_of rl si) -∗
@@ -185,54 +127,54 @@ iApply (term_meta_token with "token"); last by case: rl.
 by [].
 Qed.
 
-Definition session si : iProp :=
+Lemma unreleased_released_session si rl :
+  unreleased (si_share_of rl si) -∗
+  released_session si -∗
+  False.
+Proof.
+iIntros "#un [#rI #rR]".
+iAssert (released (si_share_of rl si)) as "r"; first by case: rl.
+by iPoseProof (term_meta_agree with "r un") as "%".
+Qed.
+
+Definition session rl si : iProp :=
   □ (▷ released_session si → public (si_key si)) ∗
-  ((public (si_init si) ∨ public (si_resp si)) ∨
-    □ (public (si_key si) → ▷ released_session si)).
+  ∃ failed,
+    term_meta (si_share_of rl si) (iso_dhN.@"failed") failed ∗
+    if failed then public (si_init si) ∨ public (si_resp si)
+    else □ (public (si_key si) → ▷ released_session si).
 
-Global Instance session_persistent si : Persistent (session si).
+Global Instance session_persistent rl si :
+  Persistent (session rl si).
 Proof. apply _. Qed.
 
-Definition session_ok si : iProp :=
-  □ (public (si_key si) ↔ ▷ released_session si).
-
-Global Instance session_ok_persistent si : Persistent (session_ok si).
-Proof. apply _. Qed.
-
-Lemma secret_session si :
+Lemma secret_session rl si :
   secret (si_init si) -∗
   secret (si_resp si) -∗
-  session si -∗
-  ◇ session_ok si.
+  session rl si -∗
+  ◇ □ (public (si_key si) ↔ ▷ released_session si).
 Proof.
-iIntros "sI sR (#comp1 & #comp2)".
-iDestruct "comp2" as "[[comp2|comp2]|comp2]".
+iIntros "sI sR (#comp1 & %failed & #failed & #comp2)".
+case: failed; eauto. iDestruct "comp2" as "[comp2|comp2]".
 - by iDestruct (secret_not_public with "sI comp2") as ">[]".
 - by iDestruct (secret_not_public with "sR comp2") as ">[]".
-- iIntros "!> !>". by iSplit.
 Qed.
 
-Lemma session_session_ok si :
-  session si -∗
-  (public (si_init si) ∨ public (si_resp si)) ∨ session_ok si.
-Proof.
-iIntros "#[#? [?|#?]]"; eauto. iRight. iModIntro. by iSplit.
-Qed.
-
-Lemma unreleased_key_secrecy si :
-  □ (¬ released_session si) -∗
-  session_ok si -∗
+Lemma unreleased_key_secrecy rl si :
+  unreleased (si_share_of rl si) -∗
+  □ (public (si_key si) ↔ ▷ released_session si) -∗
   □ (public (si_key si) ↔ ▷ False).
 Proof.
 iIntros "#un #s_k !>".
 iApply (bi.iff_trans _ (▷ released_session si)). iSplit => //.
 iSplit; last by iIntros ">[]".
-iIntros "#re !>". by iApply "un".
+iIntros "#re !>".
+by iApply unreleased_released_session.
 Qed.
 
 Lemma release_token_key_secrecy rl si :
   release_token (si_share_of rl si) -∗
-  session_ok si -∗
+  □ (public (si_key si) ↔ ▷ released_session si) -∗
   public (si_key si) -∗
   ▷ False.
 Proof.
@@ -241,40 +183,42 @@ iPoseProof ("s_k" with "p_k") as "contra".
 iModIntro. by iApply (release_token_released_session with "token").
 Qed.
 
-Lemma session_ok_compromised rl si :
-  session_ok si -∗
-  compromised si -∗
-  release_token (si_share_of rl si) -∗
-  ▷ False.
-Proof.
-iIntros "#ok [_ #comp] rel".
-iApply (release_token_key_secrecy with "rel ok comp").
-Qed.
-
 Lemma session_compromised rl si :
-  session si -∗
+  session rl si -∗
   public (si_key si) -∗
   release_token (si_share_of rl si) -∗
-  ◇ compromised si.
+  ◇ compromised_session rl si.
 Proof.
-iIntros "(#comp1 & #[[comp2|comp2]|#comp2]) #p_k rel".
-- iSplit => //. by eauto.
-- iSplit => //. by eauto.
-- iSpecialize ("comp2" with "p_k").
-  iDestruct (release_token_released_session with "rel comp2") as ">[]".
+iIntros "(#comp1 & %failed & #failed & #comp2) #p_k rel".
+case: failed; first by do !iSplit => //.
+iDestruct (release_token_key_secrecy with "rel [] p_k") as ">[]".
+iModIntro. by iSplit.
+Qed.
+
+Lemma session_not_compromised rl si :
+  session rl si -∗
+  secret (si_init si) -∗
+  secret (si_resp si) -∗
+  ◇ □ ¬ compromised_session rl si.
+Proof.
+iIntros "(#comp1 & %failed & #failed & #comp2) s_kI s_kR".
+case: failed; last first.
+{ iIntros "!> !> (_ & _ & #contra)".
+  by iPoseProof (term_meta_agree with "failed contra") as "%". }
+iDestruct "comp2" as "[comp2|comp2]".
+- iDestruct (secret_not_public with "s_kI comp2") as ">[]".
+- iDestruct (secret_not_public with "s_kR comp2") as ">[]".
 Qed.
 
 Definition msg2_pred skR m2 : iProp :=
-  ∃ ga b skI N,
+  ∃ ga b skI,
     let pkI := Spec.pkey skI in
     let pkR := Spec.pkey skR in
     let gb := TExp (TInt 0) b in
     let gab := TExp ga b in
-    let si := SessInfo skI skR ga gb gab in
-    ⌜m2 = Spec.of_list [ga; gb; pkI; Tag N]⌝ ∧
+    ⌜m2 = Spec.of_list [ga; gb; pkI]⌝ ∧
     ((public skI ∨ public skR) ∨ (public b ↔ ▷ (released ga ∧ released gb))) ∧
-    (∀ t, dh_pred b t ↔ ▷ □ iso_dh_key_share t) ∧
-    iso_dh_ready N skI skR si.
+    (∀ t, dh_pred b t ↔ ▷ □ iso_dh_pred t).
 
 Definition msg3_pred skI m3 : iProp :=
   ∃ a gb skR,
@@ -284,8 +228,7 @@ Definition msg3_pred skI m3 : iProp :=
     let gab := TExp gb a in
     let si := SessInfo skI skR ga gb gab in
     ⌜m3 = Spec.of_list [ga; gb; pkR]⌝ ∧
-    ((public skI ∨ public skR) ∨
-      □ (public (si_key si) → ▷ released_session si)).
+    ((public skI ∨ public skR) ∨ □ (public (si_key si) → ▷ released_session si)).
 
 Definition iso_dh_ctx : iProp :=
   sign_pred (iso_dhN.@"m2") msg2_pred ∗
@@ -306,7 +249,7 @@ Qed.
 
 Lemma public_dh_share a :
   minted a -∗
-  □ (∀ t, dh_pred a t ↔ ▷ □ iso_dh_key_share t) -∗
+  □ (∀ t, dh_pred a t ↔ ▷ □ iso_dh_pred t) -∗
   public (TExp (TInt 0) a).
 Proof.
 iIntros "#m_a #pred_a". rewrite public_TExpN //=; eauto.
@@ -318,8 +261,8 @@ Qed.
 Lemma public_dh_secret a b :
   minted a -∗
   minted b -∗
-  □ (∀ t, dh_pred a t ↔ ▷ □ iso_dh_key_share t) -∗
-  □ (∀ t, dh_pred b t ↔ ▷ □ iso_dh_key_share t) -∗
+  □ (∀ t, dh_pred a t ↔ ▷ □ iso_dh_pred t) -∗
+  □ (∀ t, dh_pred b t ↔ ▷ □ iso_dh_pred t) -∗
   (public (TExpN (TInt 0) [a; b]) ↔ ◇ (public a ∨ public b)).
 Proof.
 iIntros "#m_a #m_b #pred_a #pred_b".
@@ -335,14 +278,14 @@ iSplit; last first.
   - iLeft. iSplit => //. by iApply public_dh_share. }
 iIntros "[[_ #p_b] | [[_ #p_a] | (_ & contra & _)]]"; eauto.
 iPoseProof ("pred_a" with "contra") as ">%contra".
-by rewrite /iso_dh_key_share exps_TExpN /= in contra.
+by rewrite /iso_dh_pred exps_TExpN /= in contra.
 Qed.
 
 Lemma public_dh_secret' a b (P : iProp) :
   □ (public a ↔ P) -∗
-  □ (∀ t, dh_pred a t ↔ ▷ □ iso_dh_key_share t) -∗
+  □ (∀ t, dh_pred a t ↔ ▷ □ iso_dh_pred t) -∗
   □ (public b ↔ P) -∗
-  □ (∀ t, dh_pred b t ↔ ▷ □ iso_dh_key_share t) -∗
+  □ (∀ t, dh_pred b t ↔ ▷ □ iso_dh_pred t) -∗
   (public (TExpN (TInt 0) [a; b]) → ◇ P).
 Proof.
 iIntros "#s_a #pred_a #s_b #pred_b".
@@ -351,27 +294,9 @@ iIntros "[[_ #p_b] | [[_ #p_a] | (_ & contra & _)]]".
 - by iModIntro; iApply "s_b".
 - by iModIntro; iApply "s_a".
 iPoseProof ("pred_a" with "contra") as ">%contra".
-by rewrite /iso_dh_key_share exps_TExpN /= in contra.
+by rewrite /iso_dh_pred exps_TExpN /= in contra.
 Qed.
 
 End Verif.
 
-Arguments iso_dh_ctx_alloc {Σ _ _ _} E.
-
-Lemma iso_dhGS_alloc `{!heapGS Σ, !cryptisGS Σ} E :
-  ↑iso_dhN ⊆ E →
-  iso_dhGpreS Σ →
-  seal_pred_token SIGN E ={⊤}=∗ ∃ (H : iso_dhGS Σ),
-    iso_dh_ctx ∗ iso_dh_token ⊤ ∗
-    seal_pred_token SIGN (E ∖ ↑iso_dhN).
-Proof.
-iIntros "% % token".
-iMod gmeta_token_alloc as (γ_meta) "own".
-iExists (IsoDhGS _ γ_meta).
-iMod (iso_dh_ctx_alloc with "token") as "[#H ?]" => //.
-by iFrame.
-Qed.
-
-Arguments iso_dhGS_alloc {Σ _ _ E}.
-Arguments iso_dh_pred_set {Σ _} N φ E.
-Global Typeclasses Opaque session_ok.
+Arguments iso_dh_ctx_alloc {Σ _ _} E.
