examples/rpc/proofs.v
@@ -4,8 +4,8 @@ From stdpp Require Import namespaces.
 From iris.algebra Require Import agree auth csum gset gmap excl frac.
 From iris.algebra Require Import max_prefix_list.
 From iris.heap_lang Require Import notation proofmode.
-From cryptis Require Import lib cryptis primitives tactics role.
-From cryptis.examples Require Import iso_dh gen_conn conn.
+From cryptis Require Import lib term cryptis primitives tactics role.
+From cryptis.examples Require Import iso_dh conn.
 From cryptis.examples.rpc Require impl.
 From cryptis.examples.rpc.proofs Require Import base.
 
@@ -13,24 +13,16 @@ Set Implicit Arguments.
 Unset Strict Implicit.
 Unset Printing Implicit Defensive.
 
-Record handler := Handler {
-  handler_val : val;
-}.
-
-Instance repr_handler : Repr handler := handler_val.
-
 Section Proofs.
 
-Context `{!cryptisGS Σ, !heapGS Σ, !iso_dhGS Σ, !GenConn.connGS Σ, !rpcGS Σ}.
+Context `{!cryptisGS Σ, !heapGS Σ, !Conn.connGS Σ, !rpcGS Σ}.
 Notation iProp := (iProp Σ).
 
-Implicit Types (cs : GenConn.state).
+Implicit Types (cs : Conn.state).
 Implicit Types (skI skR : sign_key) (kS t : term).
 Implicit Types n : nat.
 Implicit Types γ : gname.
 Implicit Types v : val.
-
-Notation rpcN := (nroot.@"rpc").
 
 Lemma wp_connect P c skI skR :
   channel c -∗
@@ -38,22 +30,21 @@ Lemma wp_connect P c skI skR :
   ctx -∗
   minted skI -∗
   minted skR -∗
-  {{{ GenConn.failure skI skR ∨ P }}}
+  {{{ Conn.failure skI skR ∨ P }}}
     impl.connect c skI (Spec.pkey skR)
   {{{ cs, RET (repr cs);
       client_connected skI skR cs ∗
-      (compromised cs ∨ P) }}}.
+      (compromised_session Init cs ∨ P) }}}.
 Proof.
-iIntros "#? #? [#? #?] #? #? % !> P post".
-wp_lam; wp_pures. iApply wp_fupd.
-wp_apply (Conn.wp_connect with "[] [P]"); eauto 10.
+iIntros "#? #? #? #? #? % !> P post".
+wp_lam; wp_pures.
+iPoseProof (ctx_conn_ctx with "[//]") as "?".
+iApply wp_fupd.
+wp_apply (Conn.wp_connect with "[//] [//] [//] [] [] P"); eauto.
 iIntros "%cs (connected & P & rel & token)".
 iMod (resp_pred_token_alloc with "token") as "(t1 & t2 & token)";
   first solve_ndisj.
-iApply ("post" $! cs).
-iPoseProof (Conn.connected_public_key_or with "connected rel P")
-  as "(connected & rel & >P)".
-iFrame. iModIntro. iRight. by iFrame.
+iApply ("post" $! cs). iFrame. iModIntro. iRight. by iFrame.
 Qed.
 
 Lemma wp_listen c :
@@ -65,8 +56,9 @@ Lemma wp_listen c :
   {{{ ga skI, RET (ga, Spec.pkey skI)%V;
       public ga ∗ minted skI }}}.
 Proof.
-iIntros "#? #? [#? #?] % !> _ post".
-wp_lam. by iApply Conn.wp_listen.
+iIntros "#? #? #? % !> _ post".
+wp_lam. iApply Conn.wp_listen => //.
+by iApply ctx_conn_ctx.
 Qed.
 
 Lemma wp_confirm P c skI skR ga :
@@ -74,204 +66,96 @@ Lemma wp_confirm P c skI skR ga :
   cryptis_ctx -∗
   ctx -∗
   {{{ public ga ∗ minted skI ∗ minted skR ∗
-      (GenConn.failure skI skR ∨ P) }}}
+      (Conn.failure skI skR ∨ P) }}}
     impl.confirm c skR (ga, Spec.pkey skI)%V
   {{{ cs, RET (repr cs);
       server_connected skI skR cs ∗
-      (compromised cs ∨ P) }}}.
+      (compromised_session Resp cs ∨ P) }}}.
 Proof.
-iIntros "#? #ctx1 [#? #ctx2] !> %Φ (#p_ga & #m_skI & #m_skR & P) post".
-wp_lam; wp_pures. iApply wp_fupd.
-wp_apply (Conn.wp_confirm P with "[] [$P]").
-- eauto.
-- eauto.
+iIntros "#? #ctx #? !> %Φ (#p_ga & #m_skI & #m_skR & P) post".
+wp_lam; wp_pures.
+iPoseProof (ctx_conn_ctx with "[//]") as "?".
+iApply wp_fupd.
+wp_apply (Conn.wp_confirm P with "[//] [//] [//] [$P]").
+{ by eauto. }
 iIntros "%cs (conn & dis & rel & token)".
-iPoseProof (Conn.connected_public_key_or with "conn rel dis")
-  as "(conn & rel & >dis)".
 iApply "post". by iFrame.
 Qed.
 
-Lemma wp_call_gen N φ ψ skI skR cs t :
-  {{{ cryptis_ctx ∗ ctx ∗ public t ∗
-      rpc_pred N φ ψ ∗
-      connected skI skR Init cs ∗
-      client_tokens cs ∗
-      (public (si_key cs) ∨ φ skI skR cs t) }}}
-    impl.call (repr cs) (Tag N) t
-  {{{ t', RET (repr t');
-      connected skI skR Init cs ∗
-      client_tokens cs ∗
-      (public (si_key cs) ∨ ψ skI skR cs t t') ∗
-      public t' }}}.
+Lemma wp_call N φ ψ skI skR cs (ts : list term) :
+  {{{ cryptis_ctx ∗ ctx ∗
+      ([∗ list] t ∈ ts, public t) ∗
+      rpc N φ ψ ∗
+      client_connected skI skR cs ∗
+      (compromised_session Init cs ∨ φ skI skR cs ts) }}}
+    impl.call (repr cs) (Tag N) (repr ts)
+  {{{ ts', RET (repr ts');
+      client_connected skI skR cs ∗
+      (compromised_session Init cs ∨ ψ skI skR cs ts ts') ∗
+      ([∗ list] t ∈ ts', public t) }}}.
 Proof.
-iIntros "%Φ (#? & #ctx & #p_t & #N & conn & resp_pred & inv) post".
-iDestruct "ctx" as "[? ctx]".
+iIntros "%Φ (#? & #? & #p_ts & #? & conn & inv) post".
+iDestruct "conn" as "(conn & rel & resp_pred)".
 iAssert (|==>
-  (public (si_key cs) ∨ resp_pred_token cs N t) ∗
-  (public (si_key cs) ∨
-     resp_pred_token cs N t ∗ φ skI skR cs t))%I
+  (compromised_session Init cs ∨ resp_pred_token cs (ψ skI skR cs ts)) ∗
+  (compromised_session Init cs ∨
+     resp_pred_token cs (ψ skI skR cs ts) ∗
+     φ skI skR cs ts))%I
   with "[resp_pred inv]" as ">[resp_pred inv]".
 { rewrite -or_sep2.
   iDestruct "resp_pred" as "[#fail|(t1 & t2)]"; eauto.
-  iMod (resp_pred_token_update cs N t with "t1 t2") as "[t1 t2]".
+  iMod (resp_pred_token_update _ _ _ (ψ skI skR cs ts)
+         with "t1 t2") as "[t1 t2]".
   iDestruct "inv" as "[#fail|inv]"; eauto.
   iModIntro. iRight. by iFrame. }
-wp_lam. wp_pure _ credit:"c". wp_pures. wp_tag.
+wp_lam. wp_pure _ credit:"c". wp_pures.
 wp_apply (Conn.wp_send with "[] [] [$conn inv]"); eauto.
-{ by rewrite public_tag. }
-{ iDestruct "inv" as "[?|[??]]"; first by eauto. iRight.
-  iExists N, t, φ, ψ. iSplit => //. by iFrame. }
+{ iDestruct "inv" as "[(_ & ? & _)|inv]"; first by eauto. iRight.
+  by iFrame. }
 iIntros "conn". wp_pures. iApply wp_fupd.
 wp_apply (Conn.wp_recv with "[] [$conn]"); eauto.
-iIntros "%t' (conn & p_t' & inv)".
+{ by iApply ctx_resp. }
+iIntros "%ts' (conn & p_ts' & inv)".
 iApply "post".
 iDestruct "inv" as "[#inv|inv]".
-{ iFrame. iModIntro. iSplitL; iLeft; by eauto. }
+{ iPoseProof (Conn.connected_public_key with "conn rel [//]") as "#>?".
+  iFrame. iModIntro. iSplitL; by eauto. }
 iDestruct "resp_pred" as "[#fail|t1]".
-{ iFrame. iModIntro. iSplitL; iLeft; by eauto. }
-iDestruct "inv" as "(%N' & %t₀ & %φ' & %ψ' & #N' & inv & t2)".
-iPoseProof (resp_pred_token_agree with "t1 t2") as "[<- <-]".
-iPoseProof (rpc_pred_agree with "N N'") as "[_ E]".
+{ iFrame. iModIntro. iSplitL; eauto. }
+iDestruct "inv" as "(%ψ' & t2 & inv)".
+iPoseProof (resp_pred_token_agree with "t1 t2") as "#E".
+iSpecialize ("E" $! ts').
 iMod (lc_fupd_elim_later_pers with "c E") as "{E} #E".
-iRewrite ("E" $! skI skR cs t t').
-iMod (resp_pred_token_update _ rpcN (TInt 0)
-       with "t1 t2") as "t".
+iRewrite "E".
+iMod (resp_pred_token_update _ _ _ (λ _, False%I)
+       with "t1 t2") as "ts".
 by iFrame.
 Qed.
 
-Lemma wp_call N φ ψ skI skR cs t :
-  {{{ cryptis_ctx ∗ ctx ∗ public t ∗
-      rpc_pred N φ ψ ∗
-      client_connected skI skR cs ∗
-      (compromised cs ∨ φ skI skR cs t) }}}
-    impl.call (repr cs) (Tag N) t
-  {{{ t', RET (repr t');
-      client_connected skI skR cs ∗
-      (compromised cs ∨ ψ skI skR cs t t') ∗
-      public t' }}}.
-Proof.
-iIntros "%Φ (#? & #ctx & #p_t & #N & (conn & rel & tok) & inv) post".
-rewrite [in (_ ∨ φ _ _ _ _)%I]compromised_public.
-iApply wp_fupd.
-wp_apply (wp_call_gen with "[$conn $tok $inv]"); first by eauto.
-iIntros "%t' (conn & tok & res & #p_t')".
-iDestruct (Conn.connected_public_key_or with "conn rel res")
-  as "(conn & rel & >res)".
-iModIntro. iApply "post". by iFrame.
-Qed.
+Definition wf_handler Φ skI skR cs h : iProp :=
+  Conn.wf_handler
+    (release_token (si_resp_share cs) ∗ Φ)%I
+    (λ r,
+      ⌜r = #true⌝ ∗ Φ ∗
+      Conn.connected skI skR Resp cs ∗
+      release_token (si_resp_share cs) ∨
+      ⌜r = #false⌝ ∗ Φ ∗
+      public (si_key cs))%I
+    skI skR Resp cs h.
 
-Definition wf_handler Φ skI skR cs (h : handler) : iProp :=
-  □ ∀ t,
-    {{{ public t ∗
-        (public (si_key cs) ∨ rpc_msg_pred skI skR cs Init t) ∗
-        server_connected skI skR cs ∗
-        Φ }}}
-      repr h (repr cs) t
-    {{{ ob, RET (repr ob);
-        match ob : option bool with
-        | Some true =>
-            Φ ∗ server_connected skI skR cs
-        | Some false => Φ ∗ public (si_key cs)
-        | None =>
-            Φ ∗ server_connected skI skR cs ∗
-            (public (si_key cs) ∨ rpc_msg_pred skI skR cs Init t)
-        end
-    }}}.
-
-Typeclasses Opaque wf_handler.
-
-Instance persistent_wf_handler Φ skI skR cs h :
-  Persistent (wf_handler Φ skI skR cs h).
-Proof. rewrite /wf_handler. apply _. Qed.
-
-Lemma wp_handle_gen Φ N φ ψ skI skR cs (f : val) :
+Lemma wp_handle Φ N φ₁ φ₂ skI skR cs (f : val) :
   {{{
-    rpc_pred N φ ψ ∗
+    rpc N φ₁ φ₂ ∗
     ctx ∗
-    □ (∀ t : term,
-      {{{ ▷ public t ∗
-          ▷ (compromised cs ∨ φ skI skR cs t) ∗
-          release_token (si_resp_share cs) ∗
+    □ (∀ (ts : list term),
+      {{{ ▷ ([∗ list] t ∈ ts, public t) ∗
+          ▷ (compromised_session Resp cs ∨ φ₁ skI skR cs ts) ∗
           Φ }}}
-        f (repr t)
-      {{{ ores, RET (repr ores);
-          match ores : option (bool * term) with
-          | Some (continue, t') =>
-              public t' ∗
-              if continue then
-                (public (si_key cs) ∨ ψ skI skR cs t t') ∗
-                release_token (si_resp_share cs)
-              else public (si_key cs) ∨ released_session cs
-          | None => release_token (si_resp_share cs)
-          end ∗
-          Φ }}})
-  }}}
-    impl.handle_gen (Tag N) f
-  {{{ h, RET (repr h); wf_handler Φ skI skR cs h }}}.
-Proof.
-iIntros "%Ξ (#N & #ctx & #wp) post". wp_lam. wp_pures.
-iDestruct "ctx" as "(#? & #?)".
-iIntros "!>". iApply ("post" $! (Handler _)). clear Ξ.
-rewrite /wf_handler.
-iIntros "!> %t !> %Ξ (#p_t & inv_t & (conn & rel) & inv) post".
-wp_pure _ credit:"c1".
-wp_pures. wp_untag t; wp_pures; last by iApply ("post" $! None); iFrame.
-iAssert (|={⊤}=> (
-  connected skI skR Resp cs ∗
-  release_token (si_resp_share cs) ∗
-  (public (si_key cs) ∨ resp_pred_token cs N t ∗ φ skI skR cs t)))%I
-  with "[c1 conn rel inv_t]" as ">(conn & rel & inv_t)".
-{ iDestruct "inv_t" as "[#fail|inv_t]".
-  { iPoseProof (Conn.connected_public_key with "conn rel fail") as "#>?".
-    iFrame. by eauto. }
-  iFrame.
-  iDestruct "inv_t" as "(%N' & %t' & %φ' & %ψ' & %e & #N' & inv_t & token)".
-  case/Spec.tag_inj: e => /Tag_inj <- <- {N' t'}.
-  iPoseProof (rpc_pred_agree with "N N'") as "[E _]".
-  iMod (lc_fupd_elim_later_pers with "c1 E") as "{E} #E".
-  iRewrite ("E" $! skI skR cs t). iRight. by iFrame. }
-rewrite public_tag or_sep2. iDestruct "inv_t" as "[t inv_t]".
-iPoseProof (Conn.connected_public_key_or with "conn rel inv_t")
-  as "(conn & rel & >inv_t)".
-wp_apply ("wp" with "[$inv $rel inv_t]").
-{ iSplit => //. }
-iIntros ([[continue t']|]) "[res inv]"; wp_pures; last first.
-{ by iApply ("post" $! (Some true)); iFrame. }
-iDestruct "res" as "(#p_t' & inv_t')".
-iPoseProof (Conn.connected_released_session with "conn") as "#sess".
-iAssert ((if continue then (public (si_key cs) ∨ ψ skI skR cs t t')
-          else public (si_key cs)) ∗
-         (if continue then release_token (si_resp_share cs) else public (si_key cs)))%I
-  with "[inv_t']" as "[inv_t' rel]".
-{ case: continue; eauto.
-  iDestruct "inv_t'" as "[?|inv_t']"; eauto.
-  iSplit; iApply "sess"; eauto. }
-wp_apply (Conn.wp_send with "[] p_t' [$conn t inv_t']"); eauto.
-{ iDestruct "t" as "[?|t]"; eauto.
-  case: continue; eauto.
-  iDestruct "inv_t'" as "[?|inv_t']"; eauto.
-  iRight. iExists _, _, _, _. iFrame. by iFrame "#". }
-iIntros "conn". wp_pures.
-case: continue; wp_pures.
-- by iApply ("post" $! (Some true)); iFrame.
-- wp_apply (Conn.wp_free with "conn"). iIntros "_". wp_pures.
-  iApply ("post" $! (Some false)). by eauto.
-Qed.
-
-Lemma wp_handle Φ N φ ψ skI skR cs (f : val) :
-  {{{
-    rpc_pred N φ ψ ∗
-    ctx ∗
-    □ (∀ t : term,
-      {{{ ▷ public t ∗
-          ▷ (compromised cs ∨ φ skI skR cs t) ∗
-          Φ }}}
-        f (repr t)
-      {{{ ot', RET (repr ot');
-          match ot' : option term with
-          | Some t' =>
-              public t' ∗
-              (compromised cs ∨ ψ skI skR cs t t')
+        f (repr ts)
+      {{{ ts', RET (repr ts');
+          match ts' with
+          | Some ts' => ([∗ list] t ∈ ts', public t) ∗
+                        (compromised_session Resp cs ∨ φ₂ skI skR cs ts ts')
           | None => True
           end ∗
           Φ }}})
@@ -279,15 +163,39 @@ Lemma wp_handle Φ N φ ψ skI skR cs (f : val) :
     impl.handle (Tag N) f
   {{{ h, RET (repr h); wf_handler Φ skI skR cs h }}}.
 Proof.
-iIntros "%Ξ (#N & #ctx & #wp) post". wp_lam. wp_pures.
-iApply wp_handle_gen; last by eauto.
-do 2![iSplit; eauto]. clear Ξ.
-iIntros "!> %t %Ξ !> (#p_t & inv_t & rel & inv) post".
-wp_pures.
-wp_apply ("wp" with "[$inv_t $inv]") => //.
-iIntros ([t'|]) "[ot' inv]"; wp_pures; last by iApply ("post" $! None); iFrame.
-iApply ("post" $! (Some (true, t'))). iClear "wp".
-rewrite compromised_public. by iFrame.
+iIntros "%Ψ (#? & #ctx & #wp_f) post".
+iPoseProof (ctx_error with "[//]") as "#?".
+wp_lam; wp_pures.
+iApply Conn.wp_handle; last by eauto.
+iSplit => //. clear Ψ.
+iIntros "!> %ts !> %Ψ (conn & I & #p_ts & inv_ts) post".
+iDestruct "I" as "(rel & I)". wp_pures.
+iAssert (Conn.connected skI skR Resp cs ∗
+         release_token (si_resp_share cs) ∗
+         ◇ (compromised_session Resp cs ∨
+              resp_pred_token cs (φ₂ skI skR cs ts) ∗
+              φ₁ skI skR cs ts))%I
+  with "[conn rel inv_ts]" as "(conn & rel & >inv_ts)".
+{ iDestruct "inv_ts" as "[#fail|inv_ts]"; last by iFrame.
+  iPoseProof (Conn.connected_public_key with "conn rel [//]") as "#H".
+  iFrame. iMod "H" as "?". by eauto. }
+rewrite or_sep2. iDestruct "inv_ts" as "[resp_pred inv_ts]".
+wp_apply ("wp_f" with "[$]"). iIntros "%ts' (inv_ts' & inv)".
+case: ts' => [ts'|]; wp_pures; last first.
+{ wp_list.
+  wp_apply (Conn.wp_send with "[] [] [$conn]") => //.
+  { by rewrite /= public_TInt. }
+  { by iRight. }
+  iIntros "conn". wp_pures.
+  iApply "post". iModIntro. iLeft. by iFrame. }
+iDestruct "inv_ts'" as "(#p_ts' & inv_ts')".
+wp_apply (Conn.wp_send with "[] [] [inv_ts' resp_pred $conn]") => //.
+{ by iApply ctx_resp. }
+{ iDestruct "inv_ts'" as "[(_ & ? & _)|inv_ts']"; first by eauto.
+  iDestruct "resp_pred" as "[(_ & ? & _)|resp_pred]"; first by eauto.
+  iRight. iExists _. iFrame. }
+iIntros "conn". wp_pures. iApply "post". iModIntro.
+iLeft. by iFrame.
 Qed.
 
 Lemma wp_handle_close Φ skI skR cs :
@@ -295,63 +203,25 @@ Lemma wp_handle_close Φ skI skR cs :
     impl.handle_close
   {{{ h, RET (repr h); wf_handler Φ skI skR cs h }}}.
 Proof.
-iIntros "%Ξ #ctx post".
-wp_apply wp_handle_gen; last by eauto.
-iSplit; first by iDestruct "ctx" as "[??]".
-iSplit; eauto. clear Ξ.
-iIntros "!> %t %Ξ !> (#p_t & #inv_t & rel & inv) post".
-iMod (release with "rel") as "#?".
-wp_pures. iApply ("post" $! (Some (false, _))). iFrame.
-iModIntro. iSplit; eauto.
-rewrite compromised_public.
-iDestruct "inv_t" as "[?|inv_t]"; eauto.
-iRight. by iSplit.
-Qed.
-
-Lemma wp_select Φ skI skR cs handlers :
-  {{{ ctx ∗
-      server_connected skI skR cs ∗
-      Φ ∗
-      [∗ list] h ∈ handlers, wf_handler Φ skI skR cs h }}}
-    impl.select (repr cs) (repr handlers)
-  {{{ ob, RET (repr ob);
-      match ob with
-      | Some false => Φ ∗ public (si_key cs)
-      | _ => Φ ∗ server_connected skI skR cs
-      end }}}.
-Proof.
-iIntros "%Ψ (#ctx & (conn & rel) & inv & #wp_handlers) post".
-wp_lam. wp_pures. iPoseProof "ctx" as "[??]".
-wp_apply (Conn.wp_recv with "[//] [$]").
-iIntros "%m (conn & #p_m & inv_m)". wp_pures.
-wp_apply (wp_handle_close Φ skI skR cs); eauto.
-iIntros "%h #wp_h". wp_list. wp_pures.
-iApply (wp_wand _ _ _ (λ v,
-  ∃ ob : option bool,
-    ⌜v = repr ob⌝ ∗
-    match ob with
-    | Some true => Φ ∗ server_connected skI skR cs
-    | Some false => Φ ∗ public (si_key cs)
-    | None => Φ ∗ server_connected skI skR cs ∗
-              (public (si_key cs) ∨ rpc_msg_pred skI skR cs Init m)
-    end) with "[rel inv conn inv_m] [post]")%I; last first.
-{ iIntros "% (% & -> & H)". iApply "post".
-  case: ob => [[]|]; eauto.
-  by iDestruct "H" as "(?&?&?)"; iFrame. }
-clear Ψ.
-wp_apply (wp_scan_list (wf_handler Φ skI skR cs) with "[]"); last first.
-{ iSplit => //=; eauto. iExists None. by iFrame. }
-iClear "wp_handlers wp_h". clear h.
-iIntros "!> %h %Ψ !> ((%ob & %e & inv) & #wp_h) post".
-case: ob => [[]|] //= in e *.
-iDestruct "inv" as "(inv & (conn & rel) & inv_m)".
-wp_pures. rewrite /wf_handler.
-iApply ("wp_h" with "[$conn $rel $inv_m $inv]") => //.
-iIntros "!> %ob H".
-have -> : repr ob = repr (((λ b : bool, #b) <$> ob)).
-  by case: ob => [[]|].
-iApply "post". iExists ob. iFrame.
-by case: ob => [[]|].
+iIntros "%Ψ #ctx post".
+wp_apply Conn.wp_handle; last by eauto. clear Ψ.
+iPoseProof (ctx_close with "ctx") as "#?".
+iPoseProof (ctx_resp with "ctx") as "#?".
+iSplit => //.
+iIntros "!> %ts !> %Ψ (conn & inv & #p_ts & inv_ts) post".
+iDestruct "inv" as "(rel & inv)". wp_pures.
+iMod (release with "rel") as "#relS".
+iPoseProof (Conn.connected_released_session with "conn") as "#s_k".
+iAssert (|==> public (si_key cs))%I with "[inv_ts]" as ">#p_k".
+{ iDestruct "inv_ts" as "[?|[_ relC]]"; first by eauto.
+  iIntros "!>". iApply "s_k". by iSplit. }
+wp_pures. wp_list.
+wp_apply (Conn.wp_send with "[] [] [$conn]") => //.
+- by rewrite /= public_TInt.
+- by iLeft.
+iIntros "conn". wp_pures. wp_apply (Conn.wp_free with "[$conn]").
+iIntros "_". wp_pures. iApply "post".
+iModIntro. iFrame. iRight. by eauto.
 Qed.
 
 Lemma wp_server Φ skI skR cs handlers :
@@ -363,30 +233,54 @@ Lemma wp_server Φ skI skR cs handlers :
 Proof.
 iLöb as "IH".
 iIntros "%Ψ (#ctx & conn & inv & #handlers) post".
-wp_rec. wp_pures. wp_apply (wp_select with "[$conn inv]").
-{ by iFrame "#". }
-iIntros "%ob H". wp_pures.
-case: ob => [[]|]; wp_pures.
-- iDestruct "H" as "[inv server]".
-  by iApply ("IH" with "[$] post").
-- iDestruct "H" as "[inv #?]". iApply "post". by iFrame.
-- iDestruct "H" as "[inv server]".
-  by iApply ("IH" with "[$] post").
+iDestruct "conn" as "(conn & rel)".
+iPoseProof (Conn.connected_keyE with "conn") as "#(-> & -> & _)".
+wp_rec. wp_pures. wp_apply (wp_handle_close Φ _ _ cs); eauto.
+iIntros "%hc #wp_hc". wp_list.
+iAssert ([∗ list] h ∈ (hc :: handlers), wf_handler Φ _ _ cs h)%I
+  as "#wp".
+{ rewrite /=; iSplit => //. eauto. }
+iClear "wp_hc". wp_bind (Conn.select _ _).
+iApply (wp_wand with "[inv conn rel]").
+{ wp_apply (Conn.wp_select with "wp [$conn $rel $inv]"). }
+iIntros "%res Hres".
+iDestruct "Hres" as "[(-> & Hres)|(-> & Hres)]".
+- iDestruct "Hres" as "(inv & conn & rel)". wp_pures.
+  wp_apply ("IH" with "[$inv $rel $conn]") => //.
+  by do !iSplit => //.
+- iDestruct "Hres" as "(inv & rel)". wp_pures.
+  iApply "post". by iFrame.
 Qed.
 
 Lemma wp_close skI skR cs :
-  {{{ cryptis_ctx ∗ ctx ∗ client_connected skI skR cs }}}
+  {{{ ctx ∗ client_connected skI skR cs }}}
     impl.close (repr cs)
   {{{ RET #(); public (si_key cs) }}}.
 Proof.
-iIntros "%Φ (#? & #ctx & conn & rel & tok) post".
-iMod (release with "rel") as "#rel". wp_lam.
-iPoseProof "ctx" as "[? ?]".
-wp_apply (wp_call_gen with "[$conn $tok]").
-{ rewrite public_TInt. do ![iSplit; eauto]. }
-iIntros "% (conn & tok & [#? | []] & _)".
-wp_pures. wp_apply (Conn.wp_free with "conn"). iIntros "_".
-by iApply "post".
+iIntros "%Φ (#ctx & conn) post".
+iDestruct "conn" as "(conn & rel & resp_pred)".
+iPoseProof (Conn.connected_keyE with "conn") as "#(-> & -> & _)".
+wp_lam. wp_pures. wp_list.
+iMod (release with "rel") as "#relC".
+iPoseProof (ctx_close with "[//]") as "#?".
+iPoseProof (ctx_resp with "[//]") as "#?".
+rewrite or_sep2. iDestruct "resp_pred" as "[t1 t2]".
+wp_apply (Conn.wp_send with "[] [] [$conn t2]") => //.
+{ rewrite /= public_TInt. by eauto. }
+{ iDestruct "t2" as "[(_ & ? & _)|?]"; first by eauto.
+  iRight. by iFrame. }
+iIntros "conn". wp_pures.
+wp_apply (Conn.wp_recv with "[] [$]"); eauto.
+iIntros "%ts (conn & _ & inv)". wp_pure _ credit:"c".
+wp_pures. iApply wp_fupd.
+wp_apply (Conn.wp_free with "[$conn]"). iIntros "_".
+iApply "post".
+iDestruct "t1" as "[(_ & ? & _)|t1]"; eauto.
+iDestruct "inv" as "[#p_k|(% & t2 & inv)]"; eauto.
+iPoseProof (resp_pred_token_agree with "t1 t2") as "#E".
+iSpecialize ("E" $! ts). iMod (lc_fupd_elim_later_pers with "c E") as "{E} #E".
+iAssert False%I as "[]".
+by iRewrite "E".
 Qed.
 
 End Proofs.
