examples/store/proofs/base.v
@@ -6,9 +6,10 @@ From iris.algebra.lib Require Import dfrac_agree.
 From iris.base_logic.lib Require Import invariants.
 From iris.heap_lang Require Import notation proofmode.
 From iris.heap_lang.lib Require Import ticket_lock.
-From cryptis Require Import lib cryptis primitives tactics role.
+From cryptis Require Import lib term.
+From cryptis Require Import cryptis primitives tactics role.
 From cryptis.lib Require Import replica.
-From cryptis.examples Require Import iso_dh gen_conn conn rpc alist.
+From cryptis.examples Require Import iso_dh conn rpc alist.
 From cryptis.examples.store Require Import db.
 
 Set Implicit Arguments.
@@ -56,11 +57,11 @@ Proof. solve_inG. Qed.
 
 Section Defs.
 
-Context `{!cryptisGS Σ, !heapGS Σ, !iso_dhGS Σ, !GenConn.connGS Σ, !RPC.rpcGS Σ, !storeGS Σ, !tlockG Σ}.
+Context `{!cryptisGS Σ, !heapGS Σ, !Conn.connGS Σ, !RPC.rpcGS Σ, !storeGS Σ, !tlockG Σ}.
 Notation iProp := (iProp Σ).
 
 Implicit Types (si : sess_info).
-Implicit Types (cs : GenConn.state).
+Implicit Types (cs : Conn.state).
 Implicit Types (skI skR : sign_key) (kS t : term) (ts : list term).
 Implicit Types (db : gmap term term).
 Implicit Types accounts : gmap term server_client_state.
@@ -76,11 +77,11 @@ Definition db_server_ready skI skR db : iProp :=
   rep_copy skI skR dbN ∅ db.
 
 Definition db_disconnected skI skR : iProp := ∃ db,
-  (GenConn.failure skI skR ∨ db_client_ready skI skR db) ∗
+  (Conn.failure skI skR ∨ db_client_ready skI skR db) ∗
   DB.db_state skI skR dbN db.
 
 Definition db_connected' skI skR cs : iProp := ∃ db,
-  (compromised cs ∨ db_client_ready skI skR db) ∗
+  (compromised_session Init cs ∨ db_client_ready skI skR db) ∗
   DB.db_state skI skR dbN db.
 
 Definition db_connected skI skR cs : iProp :=
@@ -91,20 +92,12 @@ Lemma db_connected_ok skI skR cs :
   db_connected skI skR cs -∗
   secret skI -∗
   secret skR -∗
-  ◇ session_ok cs.
+  minted skI -∗
+  minted skR -∗
+  ◇ □ ¬ compromised_session Init cs.
 Proof.
 iIntros "(conn & _)".
 iApply (RPC.client_connected_ok with "conn").
-Qed.
-
-Lemma db_connected_ok_compromised skI skR cs :
-  db_connected skI skR cs -∗
-  session_ok cs -∗
-  compromised cs -∗
-  ▷ False.
-Proof.
-iIntros "(conn & _)".
-by iApply RPC.client_connected_ok_compromise.
 Qed.
 
 Definition db_mapsto skI skR t1 t2 : iProp :=
@@ -155,7 +148,7 @@ Qed.
 Definition server_db_connected' skI skR cs vdb : iProp := ∃ db,
   public_db db ∗
   AList.is_alist vdb (repr <$> db) ∗
-  (compromised cs ∨ db_server_ready skI skR db).
+  (compromised_session Resp cs ∨ db_server_ready skI skR db).
 
 Definition server_db_connected skI skR cs vdb : iProp :=
   RPC.server_connected skI skR cs ∗
@@ -167,7 +160,7 @@ Definition server_handler skI skR cs vdb h : iProp :=
 Definition server_db_disconnected skI skR vdb : iProp := ∃ db,
   public_db db ∗
   AList.is_alist vdb (repr <$> db) ∗
-  (GenConn.failure skI skR ∨ db_server_ready skI skR db).
+  (Conn.failure skI skR ∨ db_server_ready skI skR db).
 
 Lemma server_db_alloc skI skR vdb E :
   ↑dbN.@"server".@(skI : term) ⊆ E →
@@ -203,22 +196,21 @@ iFrame. iSplit => //. iSplit => //.
 iPureIntro. move=> *. solve_ndisj.
 Qed.
 
-Definition store_call_pred skI skR si t : iProp :=
+Definition store_call_pred skI skR si ts : iProp :=
   ∃ t1 t2 db,
-    ⌜t = Spec.of_list [t1; t2]⌝ ∗
+    ⌜ts = [t1; t2]⌝ ∗
     rep_update skI skR dbN ∅ db (<[t1 := t2]> db).
 
-Definition store_resp_pred skI skR si t t' : iProp :=
+Definition store_resp_pred skI skR si ts ts' : iProp :=
   ∃ db, rep_current skI skR dbN ∅ db.
 
 Lemma store_call t2' skI skR cs t1 t2 :
-  let P := compromised cs in
+  let P := compromised_session Init cs in
   db_connected' skI skR cs -∗
   db_mapsto skI skR t1 t2 ==∗
-  (P ∨ store_call_pred skI skR cs (Spec.of_list [t1; t2'])) ∗
+  (P ∨ store_call_pred skI skR cs [t1; t2']) ∗
   db_mapsto skI skR t1 t2' ∗
-  ∀ t', P ∨ store_resp_pred skI skR cs (Spec.of_list [t1; t2']) t' -∗
-    db_connected' skI skR cs.
+  ∀ ts', P ∨ store_resp_pred skI skR cs [t1; t2'] ts' -∗ db_connected' skI skR cs.
 Proof.
 iIntros "% (%db & ready & own_db) own_frag".
 iMod (DB.db_state_update t2' with "own_db own_frag") as "[Hstate Hmapsto]".
@@ -238,34 +230,34 @@ iExists _. iFrame. iRight. iFrame.
 Qed.
 
 Lemma store_resp skI skR cs db t1 t2 :
-  let P := compromised cs in
+  let P := compromised_session Resp cs in
   (P ∨ db_server_ready skI skR db) -∗
-  (P ∨ store_call_pred skI skR cs (Spec.of_list [t1; t2])) ==∗
+  (P ∨ store_call_pred skI skR cs [t1; t2]) ==∗
   (P ∨ db_server_ready skI skR (<[t1 := t2]>db)) ∗
-  (P ∨ store_resp_pred skI skR cs (Spec.of_list [t1; t2]) (TInt 0)).
+  (P ∨ store_resp_pred skI skR cs [t1; t2] [TInt 0]).
 Proof.
 iIntros "% [#?|ready] [#?|call]"; try by iModIntro; iSplitL; eauto.
 iDestruct "call" as "(% & % & %db' & %e & upd)".
-case/Spec.of_list_inj: e => <- <-.
+case: e => <- <-.
 iMod (rep_copy_update with "ready upd") as "(<- & ready & cur)".
 iModIntro. iSplitL "ready"; iRight; iFrame.
 Qed.
 
-Definition create_call_pred skI skR si t : iProp :=
-  ∃ t1 t2 db, ⌜t = Spec.of_list [t1; t2]⌝ ∗ ⌜db !! t1 = None⌝ ∗
+Definition create_call_pred skI skR si ts : iProp :=
+  ∃ t1 t2 db, ⌜ts = [t1; t2]⌝ ∗ ⌜db !! t1 = None⌝ ∗
     rep_update skI skR dbN ∅ db (<[t1 := t2]>db).
 
-Definition create_resp_pred skI skR si t t' : iProp :=
+Definition create_resp_pred skI skR si ts ts' : iProp :=
   ∃ db, rep_current skI skR dbN ∅ db.
 
 Lemma create_call t1 t2 skI skR cs :
-  let P := compromised cs in
+  let P := compromised_session Init cs in
   db_connected' skI skR cs -∗
   db_free_at skI skR {[t1]} ==∗
-  (P ∨ create_call_pred skI skR cs (Spec.of_list [t1; t2])) ∗
+  (P ∨ create_call_pred skI skR cs [t1; t2]) ∗
   db_mapsto skI skR t1 t2 ∗
-  ∀ t, P ∨ create_resp_pred skI skR cs (Spec.of_list [t1; t2]) t -∗
-       db_connected' skI skR cs.
+  ∀ ts, P ∨ create_resp_pred skI skR cs [t1; t2] ts -∗
+        db_connected' skI skR cs.
 Proof.
 iIntros "% (%db & ready & state) free".
 iMod (DB.db_state_create t1 t2 with "state free") as "(%db_t1 & state & mapsto)".
@@ -284,34 +276,35 @@ iExists _. iFrame. iRight. iFrame.
 Qed.
 
 Lemma create_resp skI skR cs db t1 t2 :
-  let P := compromised cs in
+  let P := compromised_session Resp cs in
   (P ∨ db_server_ready skI skR db) -∗
-  (P ∨ create_call_pred skI skR cs (Spec.of_list [t1; t2])) ==∗
+  (P ∨ create_call_pred skI skR cs [t1; t2]) ==∗
   (P ∨ db_server_ready skI skR (<[t1 := t2]>db)) ∗
-  (P ∨ create_resp_pred skI skR cs (Spec.of_list [t1; t2]) (TInt 0)).
+  (P ∨ create_resp_pred skI skR cs [t1; t2] [TInt 0]).
 Proof.
 iIntros "% [#?|ready] [#?|call]"; try by iModIntro; iSplitL; eauto.
 iDestruct "call" as "(% & % & %db' & %e & %db_t1 & upd)".
-case/Spec.of_list_inj: e => <- <- in db_t1 *.
+case: e => <- <- in db_t1 *.
 iMod (rep_copy_update with "ready upd") as "(<- & ready & cur)".
 iModIntro. iSplitL "ready"; iRight; iFrame.
 Qed.
 
-Definition load_call_pred skI skR si t1 : iProp :=
-  ∃ t2 db, ⌜db !! t1 = Some t2⌝ ∗
-           rep_update skI skR dbN ∅ db db.
+Definition load_call_pred skI skR si ts : iProp :=
+  ∃ t1 t2 db, ⌜ts = [t1]⌝ ∗ ⌜db !! t1 = Some t2⌝ ∗
+              rep_update skI skR dbN ∅ db db.
 
-Definition load_resp_pred skI skR si t1 t2 : iProp :=
-  ∃ db, ⌜db !! t1 = Some t2⌝ ∗ rep_current skI skR dbN ∅ db.
+Definition load_resp_pred skI skR si ts ts' : iProp :=
+  ∃ t1 t2 db, ⌜ts = [t1]⌝ ∗ ⌜ts' = [t2]⌝ ∗ ⌜db !! t1 = Some t2⌝ ∗
+              rep_current skI skR dbN ∅ db.
 
 Lemma load_call t1 t2 skI skR cs :
-  let P := compromised cs in
+  let P := compromised_session Init cs in
   db_connected' skI skR cs -∗
   db_mapsto skI skR t1 t2 ==∗
-  (P ∨ load_call_pred skI skR cs t1) ∗
+  (P ∨ load_call_pred skI skR cs [t1]) ∗
   db_mapsto skI skR t1 t2 ∗
-  ∀ t2', P ∨ load_resp_pred skI skR cs t1 t2' -∗
-        (P ∨ ⌜t2' = t2⌝) ∗
+  ∀ ts, P ∨ load_resp_pred skI skR cs [t1] ts -∗
+        (P ∨ ⌜ts = [t2]⌝) ∗
         db_connected' skI skR cs.
 Proof.
 iIntros "% (%db & ready & state) mapsto".
@@ -322,51 +315,53 @@ iDestruct "ready" as "[#?|(ready & cur)]".
   iIntros "% _". iSplit; eauto. iExists _. iFrame. by eauto. }
 iMod (rep_main_update db with "ready cur") as "[ready cur]".
 iModIntro. iSplitR "ready state".
-{ iRight. iExists _. iFrame. by eauto. }
-iIntros "% [#?|(%db' & %db_t1' & cur)]".
+{ iRight. iExists _, _, _. iFrame. by eauto. }
+iIntros "% [#?|(%t1' & %t2' & %db' & %et1 & -> & %db_t1' & cur)]".
 { iSplit; eauto. iFrame. by eauto. }
 iPoseProof (rep_main_current with "ready cur") as "<-".
+case: et1 => <- in db_t1' *.
 rewrite db_t1' in db_t1. case: db_t1 => ->.
 iSplit; eauto. iExists _. iFrame. iRight. iFrame.
 Qed.
 
 Lemma load_resp skI skR cs db t1 :
-  let P := compromised cs in
+  let P := compromised_session Resp cs in
   let t2 := default (TInt 0) (db !! t1) in
   (P ∨ db_server_ready skI skR db) -∗
-  (P ∨ load_call_pred skI skR cs t1) ==∗
+  (P ∨ load_call_pred skI skR cs [t1]) ==∗
   (P ∨ db_server_ready skI skR db) ∗
-  (P ∨ load_resp_pred skI skR cs t1 t2).
+  (P ∨ load_resp_pred skI skR cs [t1] [t2]).
 Proof.
 iIntros "%P /= [#?|ready] [#?|call]"; try by iModIntro; iSplitL; eauto.
-iDestruct "call" as "(%t2 & %db' & %db_t1 & upd)".
+iDestruct "call" as "(%t1' & %t2 & %db' & %e & %db_t1 & upd)".
+case: e => <- in db_t1 *.
 iMod (rep_copy_update with "ready upd") as "(<- & ready & cur)".
 rewrite db_t1 /=. iModIntro.
 iSplitL "ready"; iRight; iFrame. by eauto.
 Qed.
 
 Definition store_ctx : iProp :=
-  RPC.rpc_pred (dbN.@"store") store_call_pred store_resp_pred ∗
-  RPC.rpc_pred (dbN.@"load") load_call_pred load_resp_pred ∗
-  RPC.rpc_pred (dbN.@"create") create_call_pred create_resp_pred ∗
+  RPC.rpc (dbN.@"store") store_call_pred store_resp_pred ∗
+  RPC.rpc (dbN.@"load") load_call_pred load_resp_pred ∗
+  RPC.rpc (dbN.@"create") create_call_pred create_resp_pred ∗
   RPC.ctx.
 
 Lemma store_ctx_alloc E :
   ↑dbN ⊆ E →
-  RPC.rpc_token E -∗
+  seal_pred_token SENC E -∗
   RPC.ctx ==∗
-  store_ctx ∗ RPC.rpc_token (E ∖ ↑dbN).
+  store_ctx ∗ seal_pred_token SENC (E ∖ ↑dbN).
 Proof.
 iIntros "%sub token #?".
-rewrite RPC.rpc_token_difference => //.
+rewrite (seal_pred_token_difference _ (↑dbN)) => //.
 iDestruct "token" as "[token ?]". iFrame.
-iMod (RPC.rpc_pred_set (N := dbN.@"store") with "token")
+iMod (RPC.rpc_alloc (N := dbN.@"store") with "token")
   as "[store token]"; first solve_ndisj.
 iFrame.
-iMod (RPC.rpc_pred_set (N := dbN.@"load") with "token")
+iMod (RPC.rpc_alloc (N := dbN.@"load") with "token")
   as "[load token]"; first solve_ndisj.
 iFrame.
-iMod (RPC.rpc_pred_set (N := dbN.@"create") with "token")
+iMod (RPC.rpc_alloc (N := dbN.@"create") with "token")
   as "[create token]"; first solve_ndisj.
 by iFrame.
 Qed.
@@ -380,17 +375,17 @@ Ltac solve_ctx :=
 
 Lemma store_ctx_store :
   store_ctx -∗
-  RPC.rpc_pred (dbN.@"store") store_call_pred store_resp_pred.
+  RPC.rpc (dbN.@"store") store_call_pred store_resp_pred.
 Proof. solve_ctx. Qed.
 
 Lemma store_ctx_load :
   store_ctx -∗
-  RPC.rpc_pred (dbN.@"load") load_call_pred load_resp_pred.
+  RPC.rpc (dbN.@"load") load_call_pred load_resp_pred.
 Proof. solve_ctx. Qed.
 
 Lemma store_ctx_create :
   store_ctx -∗
-  RPC.rpc_pred (dbN.@"create") create_call_pred create_resp_pred.
+  RPC.rpc (dbN.@"create") create_call_pred create_resp_pred.
 Proof. solve_ctx. Qed.
 
 Lemma store_ctx_rpc_ctx : store_ctx -∗ RPC.ctx.
