examples/iso_dh/game.v
@@ -18,7 +18,7 @@ Existing Instance ticket_lock.
 
 Section Game.
 
-Context `{!cryptisGS Σ, !heapGS Σ, !spawnG Σ, !tlockG Σ, !iso_dhGS Σ}.
+Context `{!cryptisGS Σ, !heapGS Σ, !spawnG Σ, !tlockG Σ}.
 Notation iProp := (iProp Σ).
 
 Implicit Types t : term.
@@ -92,12 +92,12 @@ case: bcomp; wp_pures; first by iApply "post".
 by wp_apply "IH"; eauto.
 Qed.
 
-Lemma wp_check_key_secrecy c lcomp si :
+Lemma wp_check_key_secrecy c lcomp rl si :
   {{{ cryptis_ctx ∗
       channel c ∗
       inv gameN (game_inv lcomp (si_init si) (si_resp si)) ∗
       minted (si_init si) ∗ minted (si_resp si) ∗
-      session si ∗ □ (¬ released_session si) }}}
+      session rl si ∗ □ (released_session si → False) }}}
     check_key_secrecy c #lcomp (si_key si)
   {{{ RET #(); True }}}.
 Proof.
@@ -118,8 +118,7 @@ iAssert (|={⊤ ∖ ↑gameN}=> secret skI ∗ secret skR ∗
   with "[c1 s_skI s_skR]" as "{s_sk} >(s_skI & s_skR & #s_sk)".
 { iPoseProof (secret_session with "s_skI s_skR [//]")
     as "{s_sk} #>#s_sk".
-  iFrame. iIntros "!> !> #p_k".
-  by iApply unreleased_key_secrecy. }
+  iFrame. iIntros "!> !> #p_k". iApply "un". by iApply "s_sk". }
 iModIntro. iSplitR "post".
 { iExists false; iFrame. }
 wp_pures. wp_apply wp_wait_for_compromise; eauto.
@@ -135,7 +134,7 @@ Definition do_init_loop : val :=
     Fork ("loop" "c" "compromised" "set" "skI" "pkR");;
     let: "pkR'" := recv "c" in
     (guard: is_verify_key "pkR'" in
-     bind: "sk" := initiator "c" "skI" "pkR'" (Tag gameN) in
+     bind: "sk" := initiator "c" "skI" "pkR'" in
      add_fresh_lock_term_set "sk" "set";;
      if: eq_term "pkR" "pkR'" then check_key_secrecy "c" "compromised" "sk"
      else #());;
@@ -170,7 +169,6 @@ Lemma wp_do_init_loop c lcomp vset skI skR :
   channel c -∗
   cryptis_ctx -∗
   iso_dh_ctx -∗
-  iso_dh_pred gameN (λ _ _ _ _, True)%I -∗
   minted skI -∗
   minted skR -∗
   inv gameN (game_inv lcomp skI skR) -∗
@@ -179,7 +177,7 @@ Lemma wp_do_init_loop c lcomp vset skI skR :
     do_init_loop c #lcomp vset skI (Spec.pkey skR)
   {{{ RET #(); True }}}.
 Proof.
-iIntros "#chan #? #? #? #m_skI #m_skR #inv #set".
+iIntros "#chan #? #? #m_skI #m_skR #inv #set".
 iLöb as "IH". iIntros "!> %Φ _ Hpost".
 wp_rec; wp_pures; wp_apply wp_fork.
 { by iApply "IH" => //. }
@@ -189,14 +187,15 @@ wp_pures; wp_apply wp_is_verify_key.
 { by iApply public_minted. }
 iSplit; last by wp_pures; iApply "Hpost".
 iIntros "%skR' -> #m_skR'". wp_pures.
-wp_pures. wp_apply (wp_initiator false) => //.
-iIntros "%ts tsP".
+wp_pures. wp_apply (wp_initiator false) => //. iIntros "%ts tsP".
 case: ts=> [sk|] => /=; wp_pures; last by iApply "Hpost".
 iDestruct "tsP"
-  as "(%si & <- & <- & <- & #m_sk & #s_k & #? & rel & token & _)".
+  as "(%si & <- & <- & <- & #m_sk & #s_k & #? & rel & token)".
 iPoseProof (iso_dh_game_fresh Init with "token")
   as "[fresh token]"; first solve_ndisj.
-iMod (unrelease Init with "rel") as "#un".
+iMod (unrelease with "rel") as "#un".
+iAssert (□ ¬ released_session si)%I as "#?".
+{ iIntros "!> #?". by iApply (unreleased_released_session _ Init). }
 wp_apply (wp_add_fresh_lock_term_set with "[$]"). iIntros "_".
 wp_pures. wp_eq_term e; wp_pures; last by iApply "Hpost".
 move: e => /Spec.sign_pkey_inj -> {skR}.
@@ -210,7 +209,6 @@ Lemma wp_do_init c lcomp skI skR :
   channel c -∗
   cryptis_ctx -∗
   iso_dh_ctx -∗
-  iso_dh_pred gameN (λ _ _ _ _, True)%I -∗
   minted skI -∗
   minted skR -∗
   inv gameN (game_inv lcomp skI skR) -∗
@@ -218,7 +216,7 @@ Lemma wp_do_init c lcomp skI skR :
     do_init c #lcomp skI (Spec.pkey skR)
   {{{ RET #(); True }}}.
 Proof.
-iIntros "#chan #? #? #? #p_pkI #p_pkR #? %Φ _ !> post".
+iIntros "#chan #? #? #p_pkI #p_pkR #? %Φ _ !> post".
 wp_lam. wp_pures.
 wp_apply (wp_new_lock_term_set (iso_dh_game_inv Init)) => //.
 iIntros "%set #set". wp_pures.
@@ -228,7 +226,7 @@ Qed.
 Definition do_resp_loop : val :=
   rec: "loop" "c" "compromised" "set" "skR" "pkI" :=
     Fork ("loop" "c" "compromised" "set" "skR" "pkI");;
-    (bind: "res" := responder "c" "skR" (Tag gameN) in
+    (bind: "res" := responder "c" "skR" in
      let: "pkI'" := Fst "res" in
      let: "sk" := Snd "res" in
      add_fresh_lock_term_set "sk" "set";;
@@ -245,7 +243,6 @@ Lemma wp_do_resp_loop c lcomp set skI skR :
   channel c -∗
   cryptis_ctx -∗
   iso_dh_ctx -∗
-  iso_dh_pred gameN (λ _ _ _ _, True)%I -∗
   minted skI -∗
   minted skR -∗
   inv gameN (game_inv lcomp skI skR) -∗
@@ -254,7 +251,7 @@ Lemma wp_do_resp_loop c lcomp set skI skR :
     do_resp_loop c #lcomp set skR (Spec.pkey skI)
   {{{ RET #(); True }}}.
 Proof.
-iIntros "#chan #? #? #? #p_pkI #p_pkR #? #set".
+iIntros "#chan #? #? #p_pkI #p_pkR #? #set".
 iLöb as "IH". iIntros "!> %Φ _ Hpost".
 wp_rec; wp_pures; wp_apply wp_fork.
 { iApply "IH" => //. }
@@ -262,10 +259,12 @@ wp_pures. wp_apply wp_responder; first by eauto.
 iIntros "%res res".
 case: res => [[pkI' sk]|]; wp_pures; last by iApply "Hpost".
 iDestruct "res"
-  as "(%si & -> & <- & -> & #p_pkI' & #m_sk & #s_k & rel & token)".
+  as "(%si & -> & <- & <- & #p_pkI' & #m_sk & #s_k & rel & token)".
 iPoseProof (iso_dh_game_fresh Resp with "token")
   as "[fresh token]"; first solve_ndisj.
-iMod (unrelease Resp with "rel") as "#un".
+iMod (unrelease with "rel") as "#un".
+iAssert (¬ released_session si)%I as "?".
+{ iIntros "#?". by iApply (unreleased_released_session _ Resp). }
 wp_apply (wp_add_fresh_lock_term_set with "[$]"). iIntros "_".
 wp_eq_term e; wp_pures; last by iApply "Hpost".
 move: e => /Spec.sign_pkey_inj -> {skI}.
@@ -277,7 +276,6 @@ Lemma wp_do_resp c lcomp skI skR :
   channel c -∗
   cryptis_ctx -∗
   iso_dh_ctx -∗
-  iso_dh_pred gameN (λ _ _ _ _, True)%I -∗
   minted skI -∗
   minted skR -∗
   inv gameN (game_inv lcomp skI skR) -∗
@@ -285,7 +283,7 @@ Lemma wp_do_resp c lcomp skI skR :
     do_resp c #lcomp skR (Spec.pkey skI)
   {{{ RET #(); True }}}.
 Proof.
-iIntros "#? #? #? #? #? #? #? %Φ _ !> post".
+iIntros "#? #? #? #? #? #? %Φ _ !> post".
 wp_lam. wp_pures.
 wp_apply (wp_new_lock_term_set (iso_dh_game_inv Resp)) => //.
 iIntros "%set #set". wp_pures.
@@ -307,11 +305,11 @@ Definition game : val := λ: "c",
 Lemma wp_game c :
   cryptis_ctx -∗
   channel c -∗
-  iso_dh_ctx -∗
-  iso_dh_pred gameN (λ _ _ _ _, True)%I -∗
+  seal_pred_token SIGN ⊤ -∗
   WP game c {{ _, True }}.
 Proof.
-iIntros "#ctx #? #? #?"; rewrite /game; wp_pures.
+iIntros "#ctx #? sign_tok"; rewrite /game; wp_pures.
+iMod (iso_dh_ctx_alloc with "sign_tok") as "[#? _]" => //.
 wp_apply (wp_mk_sign_key with "[]"); eauto.
 iIntros "%skI #p_pkI s_skI tokenI". wp_pures.
 wp_pures. wp_apply (wp_mk_sign_key with "[]"); eauto.
@@ -333,9 +331,9 @@ Qed.
 End Game.
 
 Definition F : gFunctors :=
-  #[heapΣ; spawnΣ; cryptisΣ; tlockΣ; iso_dhΣ].
+  #[heapΣ; spawnΣ; cryptisΣ; tlockΣ].
 
-Lemma iso_dh_secure σ₁ σ₂ (v : val) t₂ e₂ :
+Lemma iso_dh_secure σ₁ σ₂ t₂ e₂ :
   rtc erased_step ([run_network game], σ₁) (t₂, σ₂) →
   e₂ ∈ t₂ →
   not_stuck e₂ σ₂.
@@ -343,9 +341,6 @@ Proof.
 have ? : heapGpreS F by apply _.
 apply (adequate_not_stuck NotStuck _ _ (λ v _, True)) => //.
 apply: cryptis_adequacy.
-iIntros (? ? c) "#ctx #chan (_ & sign & _ & _)".
-iMod (iso_dhGS_alloc with "sign") as (?) "(#? & iso_tok & _)"; eauto.
-iMod (iso_dh_pred_set gameN (λ _ _ _ _, True)%I with "iso_tok")
-  as "[#? ?]"; eauto.
-by iApply (wp_game with "ctx [//]") => //.
+iIntros (???) "#ctx #? (aenc_tok & sign_tok & ? & _)".
+by iApply (wp_game with "ctx [//] [sign_tok]") => //.
 Qed.
