examples/rpc.v
@@ -8,7 +8,3 @@ Include cryptis.examples.rpc.proofs.base.
 Include cryptis.examples.rpc.proofs.
 
 End RPC.
-
-Existing Instance RPC.repr_handler.
-Existing Instance RPC.persistent_wf_handler.
-#[global] Typeclasses Opaque RPC.wf_handler.
