examples/store/proofs/client/load.v
@@ -6,7 +6,7 @@ From iris.algebra Require Import max_prefix_list dfrac_agree.
 From iris.base_logic Require Import invariants.
 From iris.heap_lang Require Import notation proofmode.
 From cryptis Require Import lib cryptis primitives tactics role.
-From cryptis.examples Require Import iso_dh gen_conn conn rpc.
+From cryptis.examples Require Import iso_dh conn rpc.
 From cryptis.examples.store Require Import impl.
 From cryptis.examples.store.proofs Require Import base db.
 
@@ -16,8 +16,7 @@ Unset Printing Implicit Defensive.
 
 Section Verif.
 
-Context `{!cryptisGS Σ, !heapGS Σ, !iso_dhGS Σ, !GenConn.connGS Σ}.
-Context `{!RPC.rpcGS Σ, !storeGS Σ}.
+Context `{!cryptisGS Σ, !heapGS Σ, !Conn.connGS Σ, !RPC.rpcGS Σ, !storeGS Σ}.
 Notation iProp := (iProp Σ).
 
 Context `{!storeG Σ}.
@@ -38,19 +37,25 @@ Lemma wp_client_load skI skR cs t1 t2 :
       db_connected skI skR cs ∗
       db_mapsto skI skR t1 t2 ∗
       public t2' ∗
-      (compromised cs ∨ ⌜t2' = t2⌝) }}}.
+      (compromised_session Init cs ∨ ⌜t2' = t2⌝) }}}.
 Proof.
 iIntros "#? #ctx #p_t1 !> %Φ [client mapsto] post".
 iDestruct "client" as "(conn & db)".
 iMod (load_call t1 with "db mapsto") as "(load & mapsto & waiting)".
 wp_lam; wp_pures. wp_list.
 iDestruct "ctx" as "(_ & ? & _ & ctx)".
-iApply wp_fupd.
 wp_apply (RPC.wp_call with "[$conn $load]").
 { do 4!iSplit => //=; by eauto. }
-iIntros "%t' (conn & inv_t & p_t)".
-iPoseProof ("waiting" with "inv_t") as "(res & db)".
-iApply "post". by iFrame.
+iIntros "%ts' (conn & inv_ts & p_ts)". wp_pures.
+iPoseProof ("waiting" with "inv_ts") as "(res & db)".
+iApply (wp_wand _ _ _ (λ v : val, ⌜v = default (TInt 0) (head ts')⌝)%I).
+{ rewrite [repr_list ts']repr_listE.
+  by case: ts' => [|t2' ?] /=; wp_pures. }
+iIntros "% ->". iApply "post". iFrame.
+iDestruct "res" as "[#?|->]".
+- iSplit; eauto. case: ts' => [|??] //=; first by rewrite public_TInt.
+  by iDestruct "p_ts" as "[??]".
+- iSplit; eauto. by iDestruct "p_ts" as "[??]".
 Qed.
 
 End Verif.
