examples/store/proofs/client/store.v
@@ -5,7 +5,7 @@ From iris.algebra Require Import agree auth csum gset gmap excl frac.
 From iris.algebra Require Import max_prefix_list.
 From iris.heap_lang Require Import notation proofmode.
 From cryptis Require Import lib term cryptis primitives tactics role.
-From cryptis.examples Require Import iso_dh gen_conn conn rpc.
+From cryptis.examples Require Import iso_dh conn rpc.
 From cryptis.examples.store Require Import impl.
 From cryptis.examples.store.proofs Require Import base db.
 
@@ -15,13 +15,12 @@ Unset Printing Implicit Defensive.
 
 Section Verif.
 
-Context `{!cryptisGS Σ, !heapGS Σ, !iso_dhGS Σ, !GenConn.connGS Σ}.
-Context `{!RPC.rpcGS Σ, !storeGS Σ}.
+Context `{!cryptisGS Σ, !heapGS Σ, !Conn.connGS Σ, !RPC.rpcGS Σ, !storeGS Σ}.
 Notation iProp := (iProp Σ).
 
 Context `{!storeG Σ}.
 
-Implicit Types (cs : GenConn.state).
+Implicit Types (cs : Conn.state).
 Implicit Types (skI skR : sign_key) (kS t : term).
 Implicit Types n : nat.
 Implicit Types γ : gname.
@@ -39,11 +38,11 @@ Proof.
 iIntros "#? #ctx #p_t1 #p_t2 !> %Φ [client mapsto] post".
 iDestruct "client" as "(conn & db)".
 iMod (store_call t2' with "db mapsto") as "(store & mapsto & waiting)".
-wp_lam. wp_pures. wp_list. wp_term_of_list.
+wp_lam. wp_pures. wp_list.
 iPoseProof (store_ctx_store with "[//]") as "?".
 iPoseProof (store_ctx_rpc_ctx with "[//]") as "?".
 wp_apply (RPC.wp_call with "[$conn $store]").
-{ rewrite public_of_list. do 4!iSplit => //=; first by eauto. }
+{ do 4!iSplit => //=; first by eauto. }
 iIntros "%ts' (conn & store & _)". wp_pures. iApply "post".
 iFrame. by iApply "waiting".
 Qed.
