examples/store/proofs/server/create.v
@@ -5,7 +5,7 @@ From iris.algebra Require Import agree auth csum gset gmap excl frac.
 From iris.algebra Require Import max_prefix_list.
 From iris.heap_lang Require Import notation proofmode.
 From cryptis Require Import lib term cryptis primitives tactics role.
-From cryptis.examples Require Import iso_dh gen_conn conn rpc alist.
+From cryptis.examples Require Import iso_dh conn rpc alist.
 From cryptis.examples.store Require Import impl.
 From cryptis.examples.store.proofs Require Import base db.
 
@@ -15,11 +15,10 @@ Unset Printing Implicit Defensive.
 
 Section Verif.
 
-Context `{!cryptisGS Σ, !heapGS Σ, !iso_dhGS Σ, !GenConn.connGS Σ}.
-Context `{!RPC.rpcGS Σ, !storeGS Σ}.
+Context `{!cryptisGS Σ, !heapGS Σ, !Conn.connGS Σ, !RPC.rpcGS Σ, !storeGS Σ}.
 Notation iProp := (iProp Σ).
 
-Implicit Types (cs : GenConn.state).
+Implicit Types (cs : Conn.state).
 Implicit Types (skI skR : sign_key) (kS t : term).
 Implicit Types n : nat.
 Implicit Types γ : gname.
@@ -29,7 +28,7 @@ Ltac failure := iLeft; iFrame; eauto.
 
 Lemma wp_server_handle_create skI skR cs (vdb : val) :
   {{{ cryptis_ctx ∗ store_ctx }}}
-    RPC.handle (Tag $ dbN.@"create") (Server.handle_create vdb)
+    RPC.handle (Tag $ dbN.@"create") (Server.handle_create (repr cs) vdb)
   {{{ h, RET (repr h); server_handler skI skR cs vdb h }}}.
 Proof.
 iIntros "%Φ (#ctx & #ctx') post".
@@ -38,13 +37,11 @@ iPoseProof (store_ctx_rpc_ctx with "[//]") as "?".
 wp_lam. wp_pures.
 wp_apply RPC.wp_handle; last by eauto.
 do 2!iSplit => //. clear Φ.
-iIntros "!> %t !> %Φ (#p_ts & inv_ts & %db & #p_db & db & ready) post".
-wp_pures. wp_list_of_term t; wp_pures; last first.
-{ iApply ("post" $! None). by iFrame. }
+iIntros "!> %ts !> %Φ (#p_ts & inv_ts & %db & #p_db & db & ready) post".
 wp_list_match => [t1 t2 ->| ?]; wp_pures; last first.
-{ iApply ("post" $! None). by iFrame. }
-rewrite /= public_of_list /=.
-iDestruct "p_ts" as "(p_t1 & p_t2 & _)".
+{ iApply ("post" $! None). iFrame.
+  iDestruct "inv_ts" as "[fail|inv_ts]"; eauto. }
+rewrite /=. iDestruct "p_ts" as "(p_t1 & p_t2 & _)".
 wp_bind (AList.find _ _). iApply (AList.wp_find with "db") => //.
 iIntros "!> db". rewrite lookup_fmap.
 case db_t1: (db !! t1) => [t2'|]; wp_pures.
@@ -53,8 +50,8 @@ iMod (create_resp with "ready inv_ts") as "[ready inv_ts]".
 wp_bind (AList.insert _ _ _).
 iApply (AList.wp_insert with "db").
 iIntros "!> db". rewrite -fmap_insert. wp_pures.
-iApply ("post" $! (Some _)).
-iModIntro. rewrite /= public_TInt. iFrame.
+wp_list. wp_pures. iApply ("post" $! (Some _)).
+iModIntro. rewrite /= public_TInt. iFrame. iSplit => //.
 by iApply public_db_insert.
 Qed.
 
