examples/store/proofs/server/store.v
@@ -5,7 +5,7 @@ From iris.algebra Require Import agree auth csum gset gmap excl frac.
 From iris.algebra Require Import max_prefix_list.
 From iris.heap_lang Require Import notation proofmode.
 From cryptis Require Import lib term cryptis primitives tactics role.
-From cryptis.examples Require Import iso_dh gen_conn conn rpc alist.
+From cryptis.examples Require Import iso_dh conn rpc alist.
 From cryptis.examples.store Require Import impl.
 From cryptis.examples.store.proofs Require Import base db.
 
@@ -15,13 +15,12 @@ Unset Printing Implicit Defensive.
 
 Section Verif.
 
-Context `{!cryptisGS Σ, !heapGS Σ, !iso_dhGS Σ, !GenConn.connGS Σ}.
-Context `{!RPC.rpcGS Σ}.
+Context `{!cryptisGS Σ, !heapGS Σ, !Conn.connGS Σ, !RPC.rpcGS Σ}.
 Notation iProp := (iProp Σ).
 
 Context `{!storeGS Σ}.
 
-Implicit Types (cs : GenConn.state).
+Implicit Types (cs : Conn.state).
 Implicit Types (skI skR : sign_key) (kS t : term).
 Implicit Types n : nat.
 Implicit Types γ : gname.
@@ -29,7 +28,7 @@ Implicit Types v : val.
 
 Lemma wp_server_handle_store skI skR cs (vdb : val) :
   {{{ cryptis_ctx ∗ store_ctx }}}
-    RPC.handle (Tag $ dbN.@"store") (Server.handle_store vdb)
+    RPC.handle (Tag $ dbN.@"store") (Server.handle_store (repr cs) vdb)
   {{{ h, RET (repr h); server_handler skI skR cs vdb h }}}.
 Proof.
 iIntros "%Φ (#? & #ctx) post".
@@ -37,18 +36,17 @@ iPoseProof (store_ctx_store with "ctx") as "?".
 iPoseProof (store_ctx_rpc_ctx with "ctx") as "?".
 wp_lam; wp_pures. wp_apply RPC.wp_handle; last by eauto.
 do 2!iSplit => //. clear Φ.
-iIntros "!> %t !> %Φ (#p_t & inv_t & %db & #p_db & db & ready) post".
-wp_pures. wp_list_of_term t; wp_pures; last first.
-{ iApply ("post" $! None). by iFrame. }
+iIntros "!> %ts !> %Φ (#p_ts & inv_ts & %db & #p_db & db & ready) post".
+wp_pures.
 wp_list_match => [t1 t2 ->|?]; wp_pures; last first.
 { iApply ("post" $! None). by iFrame. }
-iMod (store_resp with "ready inv_t") as "[ready inv_t]".
+iMod (store_resp with "ready inv_ts") as "[ready inv_ts]".
 wp_bind (AList.insert _ _ _).
 iApply (AList.wp_insert with "db").
 iIntros "!> db". rewrite -fmap_insert.
-wp_pures. iApply ("post" $! (Some _)).
-iFrame. rewrite /= public_TInt. iModIntro. iSplit => //.
-rewrite public_of_list /=. iDestruct "p_t" as "(?&?&_)".
+wp_pures. wp_list. wp_pures. iApply ("post" $! (Some _)).
+iFrame. rewrite /= public_TInt. iModIntro.
+iDestruct "p_ts" as "(? & ? & _)". iSplit => //.
 by iApply public_db_insert.
 Qed.
 
